try omnisemantics-based StateMachineBasedExtSpec

bedrock2/src/bedrock2/StateMachineBasedExtSpec_wp.v
@@ -7,26 +7,62 @@ Section WithMem.
   Context {width: Z} {BW: Bitwidth width}
           {word: word.word width} {mem: map.map word Byte.byte}.
 
-  Context (state: Type).
+  Context {state: Type}.
   Context (is_initial_state: state -> Prop).
   Context (step:
             (* intial state *)
             state ->
-            (* input to external call: memory given away, function name, list of arguments *)
+            (* input to external call: memory given away, function name, list of args *)
             mem -> string -> list word ->
             (* output (as a arguments to a postcondition):
                memory received back, return values, new state *)
             (mem -> list word -> state -> Prop) ->
             Prop).
 
-(*
-  Fixpoint trace_leads_to_state_satisfying(t: trace)(initial: state)
-    (post: state -> Prop): Prop :=
+  Fixpoint trace_leads_to_state_satisfying(t: trace)(post: state -> Prop): Prop :=
     match t with
-    | nil => post initial
+    | nil => forall s, is_initial_state s -> post s
     | cons ((mGive, action, args), (mReceive, rets)) t' =>
-        trace_leads_to_state_satisfying initial t' (fun s =>
-          step mGive action args (fun mReceive' rets' => ??
-  Abort.
-*)
+        trace_leads_to_state_satisfying t' (fun s =>
+          step s mGive action args (fun mReceive' rets' s' =>
+            mReceive' = mReceive ->
+            rets' = rets ->
+            post s'))
+    end.
+
+  Hypothesis weaken_step: forall s mGive action args
+                                 (post1 post2: mem -> list word -> state -> Prop),
+      step s mGive action args post1 ->
+      (forall mReceive rets s', post1 mReceive rets s' -> post2 mReceive rets s') ->
+      step s mGive action args post2.
+
+  Lemma weaken_trace_leads_to_state_satisfying: forall t (post1 post2: state -> Prop),
+      trace_leads_to_state_satisfying t post1 ->
+      (forall s, post1 s -> post2 s) ->
+      trace_leads_to_state_satisfying t post2.
+  Proof.
+    induction t; simpl; intros.
+    - eauto.
+    - destruct a as (((mGive & action) & args) & (mReceive & rets)).
+      eapply IHt. 1: exact H. cbv beta.
+      intros. eapply weaken_step. 1: eassumption. cbv beta. eauto.
+  Qed.
+
+  Definition ext_spec: ExtSpec :=
+    fun (t: trace)(mGive: mem)(action: String.string)(args: list word)
+        (post: mem -> list word -> Prop) =>
+      trace_leads_to_state_satisfying t (fun s =>
+        step s mGive action args (fun mReceive rets s' => post mReceive rets)).
+
+  Lemma ext_spec_ok: ext_spec.ok ext_spec.
+  Proof.
+    unfold ext_spec. constructor.
+    - intros. (* ?? *) admit.
+    - unfold Morphisms.Proper, Morphisms.respectful, Morphisms.pointwise_relation,
+        Basics.impl.
+      intros. eapply weaken_trace_leads_to_state_satisfying. 1: eassumption.
+      cbv beta. intros. eapply weaken_step. 1: eassumption. cbv beta. clear -H. eauto.
+    - intros. admit.
+  Admitted.
+
 End WithMem.
