bedrock2/src/bedrock2/e1000_wp.v
@@ -1,0 +1,358 @@
+(*
+Formalization of a subset of the functionality of Intel's 8254x Network Interface Cards.
+
+PDF Spec:
+
+PCI/PCI-X Family of Gigabit Ethernet Controllers Software Developer's Manual
+82540EP/EM, 82541xx, 82544GC/EI, 82545GM/EM, 82546GB/EB, and 82547xx
+https://www.intel.com/content/dam/doc/manual/pci-pci-x-family-gbe-controllers-software-dev-manual.pdf
+
+These network cards were launched in the 2000s and discontinued in the 2010s, but continue to be a popular choice for virtualization, where they are often referred to as "e1000".
+ *)
+
+Require Import Coq.Strings.String.
+Require Import Coq.ZArith.ZArith.
+Require Import coqutil.Tactics.fwd.
+Require Import coqutil.Map.Interface coqutil.Map.Properties.
+Require Import coqutil.Word.Interface coqutil.Word.Bitwidth.
+Require coqutil.Map.SortedListZ.
+Require Import coqutil.Datatypes.ZList.
+Import ZList.List.ZIndexNotations. Local Open Scope zlist_scope.
+Require Import coqutil.Datatypes.RecordSetters. Import DoubleBraceUpdate.
+Require Import bedrock2.Syntax bedrock2.Semantics.
+Require Import bedrock2.StateMachineBasedExtSpec_wp.
+Require Import bedrock2.WordNotations. Local Open Scope word_scope.
+Require Import bedrock2.Map.SeparationLogic.
+Require Import bedrock2.SepLib.
+Require Import bedrock2.SepBulletPoints.
+Require Import bedrock2.RecordPredicates.
+
+(* Not part of the spec, but a convention we chose to hardcode here: *)
+Definition E1000_REGS := 0x40000000.
+
+Local Notation R x := (E1000_REGS + x) (only parsing).
+
+(* E1000 register offsets from Section 13.4 *)
+Definition E1000_RDBAL := R 0x2800. (* base addr (lo 32 bits) of receive descriptor queue *)
+Definition E1000_RDBAH := R 0x2804. (* base addr (hi 32 bits) of receive descriptor queue *)
+Definition E1000_RDLEN := R 0x2808. (* length of receive descriptor queue in bytes *)
+Definition E1000_RDH := R 0x2810. (* receive descriptor queue head *)
+Definition E1000_RDT := R 0x2818. (* receive descriptor queue tail *)
+Definition E1000_TDBAL := R 0x3800. (* base addr (lo 32 bits) of transmit descriptor queue *)
+Definition E1000_TDBAH := R 0x3804. (* base addr (hi 32 bits) of transmit descriptor queue *)
+Definition E1000_TDLEN := R 0x3808. (* length of transmit descriptor queue in bytes *)
+Definition E1000_TDH := R 0x3810. (* transmit descriptor queue head *)
+Definition E1000_TDT := R 0x3818. (* transmit descriptor queue tail *)
+
+(* Receive Descriptors (Section 3.2.3) *)
+Record rx_desc := {
+  (* 64 bits *) rx_desc_addr: Z; (* address of buffer to write to *)
+  (* 16 bits *) rx_desc_length: Z; (* length of packet received *)
+  (* 16 bits *) rx_desc_csum: Z; (* checksum *)
+  (*  8 bits *) rx_desc_status: Z;
+  (*  8 bits *) rx_desc_errors: Z;
+  (* 16 bits *) rx_desc_special: Z;
+}.
+
+(* Transmit Descriptors (Section 3.3.3) *)
+Record tx_desc := {
+  (* 64 bits *) tx_desc_addr: Z; (* address of buffer to read from *)
+  (* 16 bits *) tx_desc_length: Z; (* length of packet to be sent *)
+  (*  8 bits *) tx_desc_cso: Z; (* checksum offset: where to insert checksum (if enabled) *)
+  (*  8 bits *) tx_desc_cmd: Z; (* command bitfield *)
+  (*  8 bits *) tx_desc_status: Z;
+  (*  8 bits *) tx_desc_css: Z; (* checksum start: where to begin computing checksum *)
+  (* 16 bits *) tx_desc_special: Z;
+}.
+
+(* The Receive Queue
+
+   The queue between head (RDH) and tail (RDT) is a queue of descriptors
+   pointing to buffers that software has provided to hardware, and
+   the buffers in this queue are waiting to be filled by hardware.
+   Hardware pushes new packets at head and increases head.
+   If head reaches tail, it means there's no more space for new
+   packets, so hardware starts discarding packets.
+   Software adds new receive descriptors by setting the tail pointer to
+   one beyond the last valid descriptor that is ready to be filled.
+   Note from Section 3.2.6:
+   > HARDWARE OWNS ALL DESCRIPTORS BETWEEN [HEAD AND TAIL]. Any descriptor
+   > not in this range is owned by software.
+
+
+   The Transmit Queue
+
+   The queue between head (TDH) and tail (TDT) is a queue of descriptors
+   pointing to buffers that software has provided to hardware and that
+   hardware is supposed to sent over the network.
+   Hardware sends the packets at head and increases head.
+   Software adds new transmit descriptors at tail and increases tail, but
+   must stop before tail equals head, because that is interpreted as an
+   empty queue, not a full queue.
+   From Section 3.4:
+   > Descriptors passed to hardware should not be manipulated by software
+   > until the head pointer has advanced past them.
+*)
+
+(* Note: The Ethernet card treats memory as little-endian (see Section 2.4), and so does
+   RISC-V, but most network protocols encode multi-byte fields in big-endian order, but
+   this file is not about protocols, so everything in the current file is little-endian. *)
+
+Definition buf := list Z. (* Zs representing bytes *)
+
+Definition z_to_buf_map: map.map Z buf := SortedListZ.map buf.
+
+Record e1000_config := {
+  rx_queue_base_addr: Z; (* RDBAL/RDBAH, 64-bit total *)
+  tx_queue_base_addr: Z; (* TDBAL/TDBAH, 64-bit *)
+  rx_queue_capacity: Z; (* RDLEN / 16 *)
+  tx_queue_capacity: Z; (* TDLEN / 16 *)
+  (* Size of the receive buffers. If a packet doesn't fit, it is split into multiple
+     buffers, using multiple descriptors.
+     Hardware supports the following receive buffer sizes:
+     256 B, 512 B, 1024 B, 2048 B, 4096 B, 8192 B, 16384 B (Section 3.2.2).
+     The buffer size is controlled using RCTL.BSIZE and RCTL.BSEX (Section 13.4.22). *)
+  rx_buf_size: Z;
+}.
+
+Record e1000_state := {
+  get_e1000_config :> e1000_config;
+  rx_queue: list rx_desc;
+  tx_queue: list tx_desc;
+  rx_queue_head: Z; (* RDH *)
+  tx_queue_head: Z; (* TDH *)
+  (* We keep track of tx buffers because these remain unchanged when handed back to
+     software. Its keys are Z because the spec says that buffer addresses are always
+     64-bit addresses, even if the processor is 32-bit, and we use "word" only for
+     "word of bitwidth of processor". *)
+  tx_bufs: z_to_buf_map;
+}.
+
+Definition rx_queue_tail(s: e1000_state): Z := (* RDT *)
+  (s.(rx_queue_head) + len s.(rx_queue)) mod s.(rx_queue_capacity).
+
+Definition tx_queue_tail(s: e1000_state): Z := (* TDT *)
+  (s.(tx_queue_head) + len s.(tx_queue)) mod s.(tx_queue_capacity).
+
+Record e1000_ok(cfg: e1000_config)(s: e1000_state): Prop := {
+  config_matches: s.(get_e1000_config) = cfg;
+  RDH_bounded: 0 <= s.(rx_queue_head) < cfg.(rx_queue_capacity);
+  TDH_bounded: 0 <= s.(tx_queue_head) < cfg.(tx_queue_capacity);
+  rx_queue_bounded: len s.(rx_queue) <= cfg.(rx_queue_capacity);
+  tx_queue_bounded: len s.(tx_queue) <= cfg.(tx_queue_capacity);
+  tx_bufs_present: forall txd, List.In txd s.(tx_queue) ->
+                   exists bs, map.get s.(tx_bufs) txd.(tx_desc_addr) = Some bs /\
+                              len bs = txd.(tx_desc_length);
+}.
+
+Definition is_initial_e1000_state(s: e1000_state) :=
+  (* we don't know anything about the initial values of the registers, but we know
+     that it initially does not own any memory *)
+  s.(rx_queue) = nil /\ s.(tx_queue) = nil /\ s.(tx_bufs) = map.empty.
+
+Section WithMem.
+  Context {width: Z} {BW: Bitwidth width}
+          {word: word.word width} {mem: map.map word Byte.byte}.
+
+  (* TODO move,
+     and maybe this could be used to define array and sepapps more conveniently? *)
+  Section WithElem.
+    Context {E: Type}.
+
+    Definition layout_absolute(ps: list (word -> mem -> Prop))(addrs: list word) :=
+      seps' (List.map (fun '(p, a) => p a) (List.combine ps addrs)).
+
+    Definition layout_offsets(ps: list (word -> mem -> Prop))(offsets: list Z)(addr: word):
+      mem -> Prop :=
+      layout_absolute ps (List.map (fun ofs => word.add addr (word.of_Z ofs)) offsets).
+
+    Definition scattered_array(elem: E -> word -> mem -> Prop)
+                              (vs: list E)(addrs: list word): mem -> Prop :=
+      layout_absolute (List.map elem vs) addrs.
+
+    Definition array'(elem: E -> word -> mem -> Prop){sz: PredicateSize elem}
+                     (vs: list E): word -> mem -> Prop :=
+      layout_offsets (List.map elem vs)
+             (List.map (fun i => sz * Z.of_nat i) (List.seq O (List.length vs))).
+
+    (* starts with 0 and has same length as given list, so the last element sum
+       excludes the last element *)
+    Fixpoint prefix_sums_starting_at(s: Z)(l: list Z): list Z :=
+      match l with
+      | nil => nil
+      | cons h t => cons (s + h) (prefix_sums_starting_at (s + h) t)
+      end.
+    Definition prefix_sums: list Z -> list Z := prefix_sums_starting_at 0.
+
+    Definition sepapps'(l: list sized_predicate): word -> mem -> Prop :=
+      layout_offsets (List.map proj_predicate l) (prefix_sums (List.map proj_size l)).
+
+    Definition circular_interval(modulus start: Z)(count: nat): list Z :=
+      List.unfoldn (fun x => (x + 1) mod modulus) count start.
+
+    (* The address a passed to this predicate is the base address. The area
+       occupied by the whole buffer is a..a+modulus*sz, but there might actually
+       be nothing at a, since the slice starts at a+startIndex*sz. *)
+    Definition circular_buffer_slice(elem: E -> word -> mem -> Prop)
+      {sz: PredicateSize elem}(modulus startIndex: Z)(vs: list E): word -> mem -> Prop :=
+      layout_offsets (List.map elem vs)
+             (List.map (Z.mul sz) (circular_interval modulus startIndex (List.length vs))).
+  End WithElem.
+
+  Definition rx_desc_t(r: rx_desc): word -> mem -> Prop := .**/
+    typedef struct __attribute__ ((__packed__)) {
+      uint64_t rx_desc_addr;
+      uint16_t rx_desc_length;
+      uint16_t rx_desc_csum;
+      uint8_t rx_desc_status;
+      uint8_t rx_desc_errors;
+      uint16_t rx_desc_special;
+    } rx_desc_t;
+  /**.
+
+  Definition tx_desc_t(r: tx_desc): word -> mem -> Prop := .**/
+    typedef struct __attribute__ ((__packed__)) {
+      uint64_t tx_desc_addr;
+      uint16_t tx_desc_length;
+      uint8_t tx_desc_cso;
+      uint8_t tx_desc_cmd;
+      uint8_t tx_desc_status;
+      uint8_t tx_desc_css;
+      uint16_t tx_desc_special;
+    } tx_desc_t;
+  /**.
+
+(* Operations:
+
+- receive-related:
+  + read RDH: new RDH can be anywhere between old RDH (incl) and RDT (excl),
+    we receive the memory chunk for each descriptor between old and new RDH,
+    as well as the buffers pointed to by them, which contain newly received packets
+  + write RDT: software may set new RDT to anywhere between old RDT (incl) and
+    RDH (excl, because otherwise queue considered empty), and by doing so, abandons
+    the memory chunks corresponding to these descriptors and the buffers pointed to
+    by them, thus providing more space for hardware to store received packets
+- transmit-related:
+  + read TDH: new TDH can be anywhere between old TDH (incl) and TDT (excl),
+    increased TDH means some packets were sent, and we get back the memory chunk
+    for each descriptor between old and new TDH, as well as the buffers pointed to
+    by them, so we can start reusing these descriptors & buffers for new packets
+  + write TDT: software may set new TDT to anywhere between old TDT (incl) and
+    TDH (excl, because otherwise queue considered empty), and by doing so, indicates
+    that between old and new TDT, there are new packets to be sent, and yields
+    the descriptor chunks and the buffers pointed to by them to hardware
+*)
+
+  Definition read_RDH(s: e1000_state)(post: word -> e1000_state -> Prop): Prop :=
+    False. (* TODO add is mGive and mReceive *)
+
+  Definition e1000_step_fun:
+    e1000_state ->
+    ((mem * String.string * list word) * (mem * list word)) ->
+    e1000_state ->
+    Prop :=
+    fun s '((mGive, action, args), (mReceive, rets)) s' =>
+      if String.eqb action "MMIOREAD"%string then
+        match args with
+        | cons addr nil =>
+            if \[addr] =? E1000_RDH then False
+            else False
+        | _ => False
+        end
+      else if String.eqb action "MMIOWRITE" then
+        match args with
+        | cons addr (cons value nil) =>
+            if \[addr] =? E1000_RDT then False
+            else False
+        | _ => False
+        end
+      else False.
+
+  Local Open Scope sep_bullets_scope.
+  Local Open Scope string_scope.
+
+  Inductive e1000_step:
+    (* intial state *)
+    e1000_state ->
+    (* input to external call: memory given away, function name, list of args *)
+    mem -> string -> list word ->
+    (* output (as a arguments to a postcondition):
+       memory received back, return values, new state *)
+    (mem -> list word -> e1000_state -> Prop) ->
+    Prop :=
+  (* read RDH: new RDH can be anywhere between old RDH (incl) and old RDT (excl),
+     we receive the memory chunk for each descriptor between old and new RDH,
+     as well as the buffers pointed to by them, which contain newly received packets *)
+  | read_RDH_step: forall s (post: mem -> list word -> e1000_state -> Prop),
+      (forall mRcv new_RDH (packets: list buf),
+          len packets <= len s.(rx_queue) ->
+          \[new_RDH] = (s.(rx_queue_head) + len packets) mod s.(rx_queue_capacity) ->
+          (* we get back a (wrapping) slice of the rx queue as well as the corresponding
+             buffers *)
+          <{ * circular_buffer_slice rx_desc_t s.(rx_queue_capacity) s.(rx_queue_head)
+                                     s.(rx_queue)[:len packets] /[s.(rx_queue_base_addr)]
+             * scattered_array (array (uint 8) s.(rx_buf_size)) packets
+                 (List.map (fun d => /[d.(rx_desc_addr)]) s.(rx_queue)[:len packets])
+            }> mRcv ->
+          post mRcv [|new_RDH|]
+            s{{ rx_queue := s.(rx_queue)[:len packets];
+                rx_queue_head := (s.(rx_queue_head) + len packets) mod
+                                 s.(rx_queue_capacity) }}) ->
+      e1000_step s map.empty "MMIOREAD" [| /[E1000_RDH] |] post.
+
+  Global Instance ext_spec: ExtSpec :=
+    StateMachineBasedExtSpec_wp.ext_spec is_initial_e1000_state e1000_step.
+
+  Global Instance ext_spec_ok: ext_spec.ok ext_spec.
+  Proof.
+    apply StateMachineBasedExtSpec_wp.ext_spec_ok.
+    intros.
+  Admitted.
+
+  Definition trace_state_satisfies: trace -> (e1000_state -> Prop) -> Prop :=
+    trace_leads_to_state_satisfying is_initial_e1000_state e1000_step.
+
+  Context {locals: map.map String.string word}.
+
+  (* TODO move to bedrock2.Semantics *)
+  Lemma exec_interact_cps: forall e binds action arges args t m l
+                                  (post: trace -> mem -> locals -> Prop) mKeep mGive,
+      map.split m mKeep mGive ->
+      eval_call_args m l arges = Some args ->
+      ext_spec t mGive action args (fun mReceive resvals =>
+          exists l', map.putmany_of_list_zip binds resvals l = Some l' /\
+          forall m', map.split m' mKeep mReceive ->
+          post (cons ((mGive, action, args), (mReceive, resvals)) t) m' l') ->
+      exec e (cmd.interact binds action arges) t m l post.
+  Proof. intros. eauto using exec.interact. Qed.
+
+  (* read RDH: new RDH can be anywhere between old RDH (incl) and old RDT (excl),
+     we receive the memory chunk for each descriptor between old and new RDH,
+     as well as the buffers pointed to by them, which contain newly received packets *)
+  Lemma wp_read_RDH: forall e cfg old_RDH old_rx_descs t m l r
+                            (post: trace -> mem -> locals -> Prop),
+      trace_state_satisfies t (fun s => e1000_ok cfg s /\
+         s.(rx_queue_head) = old_RDH /\ s.(rx_queue) = old_rx_descs) ->
+      (forall (m' mRcv: mem) (packets: list buf),
+          map.split m' mRcv m ->
+          len packets <= len old_rx_descs ->
+          let new_RDH := /[(old_RDH + len packets) mod cfg.(rx_queue_capacity)] in
+          (* we get back a (wrapping) slice of the rx queue as well as the corresponding
+             buffers *)
+          <{ * circular_buffer_slice rx_desc_t cfg.(rx_queue_capacity) old_RDH
+                                     old_rx_descs[:len packets] /[cfg.(rx_queue_base_addr)]
+             * scattered_array (array (uint 8) cfg.(rx_buf_size)) packets
+                   (List.map (fun d => /[d.(rx_desc_addr)]) (old_rx_descs[:len packets]))
+          }> mRcv ->
+          post (cons ((map.empty, "MMIOREAD", [| /[E1000_RDH] |]), (mRcv, [|new_RDH|])) t)
+               m' (map.put l r new_RDH)) ->
+      exec e (cmd.interact [|r|] "MMIOREAD" [|expr.literal E1000_RDH|]) t m l post.
+  Proof.
+    intros.
+    unfold trace_state_satisfies in *.
+    eapply exec_interact_cps.
+    3: {
+      unfold ext_spec, StateMachineBasedExtSpec_wp.ext_spec.
+  Abort.
+
+End WithMem.
